@prefix owl: <http://www.w3.org/2002/07/owl#>.
@prefix rdf: <http://www.w3.org/1999/02/22-rdf-syntax-ns#>.
@prefix rdfs: <http://www.w3.org/2000/01/rdf-schema#>.
@prefix xsd: <http://www.w3.org/2001/XMLSchema#>.
@prefix foaf: <http://xmlns.com/foaf/0.1/>.
@prefix vs: <http://www.w3.org/2003/06/sw-vocab-status/ns#>.
@prefix tl: <http://purl.org/NET/c4dm/timeline.owl#>.
@prefix event: <http://purl.org/NET/c4dm/event.owl#>.
@prefix mo: <http://purl.org/ontology/mo/>.
@prefix co: <http://purl.org/ontology/chord/>.
@prefix tonality: <http://purl.org/ontology/tonality/>.
@prefix int: <http://purl.org/ontology/tonality/interval/>.
@prefix scale: <http://purl.org/ontology/tonality/scale/>.
@prefix mode: <http://purl.org/ontology/tonality/mode/>.
@prefix key: <http://purl.org/ontology/tonality/key/>.
@prefix tuning: <http://purl.org/ontology/tuning/>.
@prefix dc: <http://purl.org/dc/elements/1.1/>.
@prefix dcterms: <http://purl.org/dc/terms/>.
@prefix note: <http://purl.org/ontology/chord/note/>.
@prefix daml: <http://www.daml.org/2001/03/daml+oil#> .
@prefix af: <http://purl.org/ontology/af/> .

<> 
	a owl:Ontology;
	dc:title "The Tonality ontology";
	rdfs:label "The Tonality ontology";
	rdfs:comment """

		Sound is a physical phenomenom consisting of the variation of pressure produced by an acoustic wave. This physical phenomenom is perceived by humans by means of the earing. Physical properties of the sound (acoustic features) are perceived as psychological features (timbre, pitch, duration, loudness...), which depend on the earing response and the brain, producing mental states in the receptor.

		Music is the high-level human production of the sound that does not convey information but is based on the effects that the sound produces in ourselves. Music "languages" and systems are built to categorize and organize the sound domain. Musical notes are the categories we use to express and perceive music as phonemes are the acoustical categories that allow us to convey information. As it happens for the phonemes, real note events are not equal but they can be distinguised by physical properties that affect our perception producing a wide range of variations.

		The perception of the fundamental frequency of the sound (pitch) is of particular interest in music as it is the basis for the construction of musical systems and a really important factor of music production. Perceptios are combined in the brain in complex cognitive constructions. Generally speaking, cognitive structures related to pitch are referred as Tonality.

		The Tonality Ontology is a specific-domain ontology that describes tonal content information of musical works and expressions. This ontology has been designed in the Music Ontology framework and closely collaborates with the Audio Features Ontology.
		
		This document is in a testing stage. Contribution can be made through the Music Ontology community at http://wiki.musicontology.com/

	""";
	dc:creator "David Pastor Escuredo";
        foaf:maker "David Pastor Escuredo";
        dc:date "$Date: 2008/10/04 18:05:11 $";
	.

# People
#<http://yo> a foaf:Person.

# Status of terms


#####################
#### CLASSES ########
#####################

tonality:Pitch
	a owl:Class;
	rdfs:label "Pitch";
	rdfs:comment """
		Pitch is the perception of the fundamental frequency of a sound. Each played note (a real event) owns physical properties that can be viewed also as human perceptions. The matching between physical and psycological properties is not linear either a one-to-one set of relationships. Tonality is about pitches perception and relationships within a meaningful expression. Pitches are represented by symbols (symbolic notes) used to categorize our perception of sounds as a musical vocabulary.
	""";
	vs:term_status "unstable";
	.

tonality:PitchClass
	a owl:Class;
	rdfs:label "Pitch Class";
	rdfs:subClassOf tonality:Pitch;
	rdfs:comment """
		Generalization of pitch families where octave, enharmonic and inversion equivalencies are assumed. Equivalent pitches in different octaves are wrapped in the same class. Thus, different frequencies fall in the same musical category.
	""";
	vs:term_status "unstable";
	.
	
tonality:Interval
	a owl:Class;	
	rdfs:label "Interval";
	rdfs:comment """
		Distance in pitch between two different sounds. Intervals can be referred to distinct tuning systems and measured with different metrics. Intervals establish the relationships among pitches, so they are the basic elements to build musical structures. The interval corresponds physically to a frequency distance, but the psychological distance between two pitches is not derived from it.
	""";
	vs:term_status "stable";	
	.

tonality:IntervalClass
	a owl:Class;
	vs:term_status "unstable";
	rdfs:subClassOf tonality:Interval;
	rdfs:label "Interval Class";
	rdfs:comment """
		Generalization if interval classes representing the between two unordered pitch classes where octave, enharmonic and inversional equivalencies are assumed. There are then 7 classes (0-6) representing distances from the minimum to the maximum value possible within the octave. 
	""";
	.

tonality:Set
	a owl:Class;
	vs:term_status "unstable";
	rdfs:label "Set"
	rdfs:comment """
		Music set formed of an unordered bunch of musical entities. For example {C, D, E, F, G, A, B} is the diatonic set for the key C major.
	""";
	.

tonality:Scale
	a owl:Class;
	rdfs:label "Scale";
	rdfs:comment """
		Musical sets can be ordered setting a tonic or a final pitch, forming scales. Then, each member of the set plays a role in the scale in respect of the tonic. Therefore, scales are ordered sequences of pitches in respect of a tonic. A progression of notes along a fragment of a musical work can be also considered a scale with a final note, but in this case those notes belongs to a more elementary structure understood as a scale in the first sense.
	""";
	vs:term_status "stable";
	.

tonality:Mode
	a owl:Class;
	rdfs:label "Mode";
	rdfs:comment """
		Sets can be ordered in several ways forming different scales. The ways we can order a set are the "Modes", so each scale has a particular shape which really describes it. From a tonic and a mode we can generate a scale.
	""";
	vs:term_status "stable";
	.

tonality:KeyMode
	a owl:Class;
	rdfs:label "Key Mode";
	rdfs:subClassOf tonality:Mode;
	rdfs:comment """
		Minor or major modes of a key.
	""";
	vs:term_status "testing";
	.

tonality:Degree
	a owl:Class;
	rdfs:label "Degree";
	rdfs:comment """
		Ordered sequences owns pitch relationships among their members. Each member is a degree and its tonal and harmonic properties depend on its position in the sequence.
	""";
	vs:term_status "unstable";
	.

tonality:Key
	a owl:Class;
	rdfs:label "Key";
	rdfs:comment """
		Keys are a musical element mainly defined and useful within the western music. It is quite difficult to give a precise definition of key that everybody agrees with. In the Tonality Ontology, the key is seen as higher abstraction of scales only meaningful in traditional tonal music.
Keys own a tonic and a mode (normally major and minor) and are used as pattern for stable compositions. Note that the minor mode of a key is a mixture of the minor mode of the diatonic set and the harmonic and melodic minor scales.
On the other hand, keys are very important in harmony. A chord progression establish a key through a fragment and vice-versa the key establish the harmonic function of a set of chords.
	""";
	vs:term_status "unstable";
	.
		
tonality:TonalSegment
	a owl:Class;
	rdfs:subClassOf af:MusicSegment;
	rdfs:label "Tonal Segment";
	rdfs:comment """
		 A tonal classifier of one particular segment of the timeline of a signal with specific tonal content defining tonal regions. Each tonal element associated with the event is considered as a factor. The audio features ontology owns a wider range of classifiers related to tonality and other features.
	""";
	vs:term_status "stable";
	.

##############################
###DEFINED PROPERTIES#########
##############################

#INTERVAL RELATED

tonality:steps a owl:FunctionalProperty;
        vs:term_status "unstable";
        rdfs:label "steps";
        rdfs:comment "Measure for intervals in equally-tempered systems";
        rdfs:domain tonality:Interval;
	rdfs:domain tonality:IntervalClass;
        rdfs:range xsd:decimal;
	a owl:DatatypeProperty;
        .

tonality:semitones a owl:FunctionalProperty;
        vs:term_status "unstable";
        rdfs:label "semitones";
        rdfs:comment "Convenience measure in EDO systems. Treated as distance it doesn't represent the real tonal distance but a frequency distance.";
        rdfs:domain tonality:Interval;
	rdfs:domain tonality:IntervalClass;
	rdfs:range xsd:integer;
	rdfs:equivalentProperty co:semitone_interval;
	a owl:DatatypeProperty;
        .

tonality:scale_steps a owl:FunctionalProperty;
        vs:term_status "unstable";
        rdfs:label "scale steps";
        rdfs:comment """
		Steps of the scale comprised in the interval. This is used to characterized general intervals and relate specific intervals to the a certain degree.
	""";
        rdfs:domain tonality:Interval;
	rdfs:range xsd:integer;
	a owl:DatatypeProperty;
        .

tonality:ratio a owl:FunctionalProperty;
	vs:term_status "unstable";
	rdfs:label "ratio";
	rdfs:comment "Measure of intervals in Just Intonation system as a ratio of the frequencies (simple rationale numbers).";
	rdfs:domain tonality:Interval;
	a owl:DatatypeProperty;
	.

tonality:comparable_ratio a owl:FunctionalProperty;
	vs:term_status "unstable";
	rdfs:label "comparable ratio";
	rdfs:comment "Closest ratio in a Just Intonation tuning for a given equally-tempered interval. (This is actually very optional).";
	rdfs:domain tonality:Interval;
	a owl:DatatypeProperty;
	.	

tonality:tuning a owl:FunctionalProperty;
	vs:term_status "unstable";
	rdfs:label "in tuning";
	rdfs:comment """
		The tuning system in which we consider the interval. Through this property we do not restric the interval definition to an equally temperament but to any temperament and division of the octave.
	""";
	rdfs:domain tonality:Interval;
	rdfs:range tuning:TuningSystem;
	a owl:ObjectProperty;
	.

tonality:cents a owl:FunctionalProperty;
	vs:term_status "unstable";
	rdfs:label "cents";
	rdfs:comment """
		Cents measurement: 1200×log2(f2/f1). This value is used to compare the size of intervals.
	""";
	rdfs:domain tonality:Interval;
	rdfs:range xsd:decimal;
	a owl:DatatypeProperty;
	.

tonality:just_cents a owl:FunctionalProperty;
	vs:term_status "unstable";
	rdfs:label "just cents";
	rdfs:comment """
		Just cents does not represent the real cents of the interval but the cents value of the comparable ratio for a equal-tempered interval. This is very optional as well in interval definition.
	""";
	rdfs:domain tonality:Interval;
	rdfs:range xsd:decimal;
	a owl:DatatypeProperty;
	.
	
tonality:interval_class a owl:SymmetricProperty;
	vs:term_status "unstable";
	rdfs:label "of interval class";
	rdfs:comment "The Interval Class (0-6) which the interval belongs to according to the semitones property";
	rdfs:domain tonality:Interval;
	rdfs:range tonality:IntervalClass;
	a owl:ObjectProperty;
	.

tonality:inversion a owl:SymmetricProperty;
	vs:term_status "unstable";
        rdfs:label "inversion";
        rdfs:comment "This property links an interval with its inversion. Major second is the inversion of minor seventh.";
	rdfs:range tonality:Interval;
        rdfs:domain tonality:Interval;
	a owl:ObjectProperty;
        .

tonality:enharmonically_equivalent a owl:SymmetricProperty;
	vs:term_status "unstable";
        rdfs:label "enharmonically_equivalent";
        rdfs:comment """
                Two intervals are enharmonically equivalent when they express the same pitch distance but as different general intervals, so they have the same number of semitones but different number of scale steps. Enharmony is a general musical property which states that two different musical elements has the same acoustic value.
        """;
	rdfs:range tonality:Interval;
        rdfs:domain tonality:Interval;
	a owl:ObjectProperty;
        .

tonality:simple_interval a owl:FunctionalProperty;
        vs:term_status "unstable";
        rdfs:label "close interval";
        rdfs:comment """
               In equal temperaments compound intervals (bigger than a octave) are indeed a close interval and n octaves. This property relates an compound interval like minor ninth with its close version minor second. 
        """;
        rdfs:domain tonality:Interval;
	rdfs:range tonality:Interval;
	a owl:ObjectProperty;
        .

tonality:octaves a owl:FunctionalProperty;
	vs:term_status "unstable";
        rdfs:label "octaves";
        rdfs:comment "Number of octaves comprised in an compound interval.";
        rdfs:domain tonality:Interval;
	rdfs:range xsd:integer;
	a owl:DatatypeProperty;
	.

tonality:strength a owl:FunctionalProperty;
	vs:term_status "unstable";
        rdfs:label "strength";
        rdfs:comment """
               This property expresses the stability of an interval given its tuning. Although is very difficult to state that a certain interval is stable or not.
        """;
        rdfs:domain tonality:Interval;
	a owl:DatatypeProperty;
        .

tonality:interval a owl:ObjectProperty;
	vs:term_status "unstable";
	rdfs:label "interval";
	rdfs:comment """
		This property allows to link an interval to some other structure. So far we define intervals for Scale, Degree (which link it to a Scale or a Key) and Chord.
	""";
	rdfs:domain tonality:Scale;
	rdfs:domain tonality:Degree;
	rdfs:domain co:Chord;
	rdfs:domain tonality:Set;
	rdfs:range tonality:Interval;
	.

#DEGREE RELATED

tonality:degree_name a owl:FunctionalProperty;
	vs:term_status "unstable";
	rdfs:label "degree name";
	rdfs:comment """
		Property that expresses the name of the degree which normally will convey implicitly its harmonic functionality. We declare a specific property for this instead of using any other name property.
	""";
	rdfs:domain tonality:Degree;
	a owl:DatatypeProperty;
	.

tonality:degree_position a owl:FunctionalProperty;
	vs:term_status "unstable";
	rdfs:label "degree position";
	rdfs:comment "Position of the degree within the scale which will determine its functionality.";
	rdfs:domain tonality:Degree;
	rdfs:range xsd:integer;
	a owl:DatatypeProperty;
	.

tonality:pitch_class a owl:FunctionalProperty;
	vs:term_status "unstable";
	rdfs:label "pitch class";
	rdfs:comment """
		This property expresses the same information than note except for the difference we consider between note and pitch class. This should be better considered.
	""";
	a owl:ObjectProperty;
	rdfs:domain tonality:Degree;
	rdfs:domain tonality:Pitch;
	rdfs:range tonality:PitchClass;
	.

tonality:pitch a owl:FunctionalProperty;
	vs:term_status "unstable";
	rdfs:label "pitch";
	rdfs:comment """
		Associates the degree to a total pitch which is determined by a note in a specific octave. This is only necessary when the tuning system is not equally tempered so pitches can not be easily infered from octave to octave (non-octave equivalency).
	""";
	rdfs:domain tonality:Degree;
	rdfs:range tonality:Pitch;
	a owl:ObjectProperty;
	.

tonality:octave a owl:FunctionalProperty;
	vs:term_status "unstable";
	rdfs:label "octave";
	rdfs:comment "Specify the concrete pitch in a particular octave. Eg: A in the 3rd octave.";
	rdfs:domain tonality:Pitch;
	rdfs:range xsd:integer;
	a owl:DatatypeProperty;
	.

tonality:frequency a owl:FunctionalProperty;
	vs:term_status "unstable";
	rdfs:label "frequency";
	rdfs:comment "Express the real frequency of the pitch.";
	rdfs:domain tonality:Degree;
	rdfs:domain tonality:Pitch;
	rdfs:range  xsd:decimal;
	a owl:DatatypeProperty;
	.

tonality:owned_chord a owl:ObjectProperty;
	vs:term_status "unstable";
	rdfs:label "owned chord";
	rdfs:comment """
		This property allows to associate chords to each of the degrees of the key describing the harmonic properties of the tonality. We will associate 7th chords as standard, but any chord with the same functionality would be valid as well. Other chords will be then borrowed from a key not actually present or produced by the use of a chromatic interval (to avoid a tritone for example). See borrowed_chord
	""";
	rdfs:domain tonality:Degree;
	rdfs:range co:Chord;
	.

tonality:borrowed_chord a owl:ObjectProperty;
	vs:term_status "unstable";
	rdfs:label "borrowed chord";
	rdfs:comment """
		Some chords owned by a key (infered for the underlying scale) are not very stable so some alterations are normally present to obtain more stability like the V degree of the relative minor key. Some degrees substitute its seventh owned interval by some other seventh interval from the parallel key giving a borrowed chord but still diatonic (altered chords came from non diatonic intervals). An important case is also the alteration of the dominant degree of the minor key to obtain a tritone producing the harmonic minor scale (can be seen as a chord borrowed from the major relative key). Borrowed chords are normally used in a key (minor or major), however other chords can be used while playing in a particular key. These chords should be classified as other tonal events (see audio features ontology).
	""";
	rdfs:domain tonality:Degree;
	rdfs:range co:Chord;
	.

tonality:degree a owl:ObjectProperty;
	vs:term_status "unstable";
	rdfs:label "degree";
	rdfs:comment "Binds a degree resource to a structure.";
	rdfs:domain tonality:Key;
	rdfs:domain tonality:Scale;
	rdfs:domain tonality:Mode;
	rdfs:range tonality:Degree;
	.

#SCALES, KEYS AND MODES

tonality:mode a owl:ObjectProperty;
	vs:term_status "unstable";
	rdfs:label "mode";
	rdfs:comment """
		Mode of a scale (its shape). The scale is well defined by a tonic or reference note and a mode (different organizations of a set). Modes are also used to characterize keys, but in a slightly different way. There are only two modes for keys (major and minor) which actually do not wholy correspond to the minor and major scale modes. Both structures can be defined by an ordered sequence of notes.
	""";
	rdfs:domain tonality:Scale;
	rdfs:domain tonality:Key;
	rdfs:range tonality:Mode;
	.

tonality:tonic a owl:FunctionalProperty;
	a owl:ObjectProperty;
	vs:term_status "unstable";
	rdfs:label "tonic";
	rdfs:comment "Sets the tonic of a key or scale if the first degree is not bound to a note.";
	rdfs:domain tonality:Key;
	rdfs:domain tonality:Scale;
	rdfs:range tonality:Pitch;	
	.

tonality:num_degrees a owl:FunctionalProperty;
	vs:term_status "unstable";
	rdfs:label "number of degrees";
	rdfs:comment "Number of steps in a scale.";
	rdfs:domain tonality:Scale;
	rdfs:range xsd:integer;
	a owl:DatatypeProperty;
	.

tonality:scale a owl:ObjectProperty;
	vs:term_status "unstable";
	rdfs:label "scale";
	rdfs:comment "Binds a scale to other structures.";
	rdfs:domain tonality:Key;
	rdfs:range tonality:Scale;
	.

##############
#Individuals##
##############

####################Interval Class individuals##############

int:ic0 a tonality:IntervalClass;
	rdfs:label "Interval class 0";
	vs:term_status "unstable";
	rdfs:comment "The interval class 0 for unison an octave.";
	tonality:semitones 0;
	.

int:ic1 a tonality:IntervalClass;
	rdfs:label "Interval class 1";
	vs:term_status "unstable";
	rdfs:comment "minor second and major seventh and enharmonically_equivalents.";
	tonality:semitones 1;
	.

int:ic2 a tonality:IntervalClass;
	vs:term_status "unstable";
	rdfs:label "Interval class 2";
	rdfs:comment "major second and minor seventh and enharmonically_equivalents.";
	tonality:semitones 2;
	.

int:ic3 a tonality:IntervalClass;
	rdfs:label "Interval class 3";
	vs:term_status "unstable";
	rdfs:comment "minor third and major sixth and enharmonically_equivalents.";
	tonality:semitones 3;
	.

int:ic4 a tonality:IntervalClass;
	rdfs:label "Interval class 4";
	vs:term_status "unstable";
	rdfs:comment "major third and minor sixth and enharmonically_equivalents.";
	tonality:semitones 4;
	.

int:ic5 a tonality:IntervalClass;
	rdfs:label "Interval class 5";
	vs:term_status "unstable";
	rdfs:comment "perfect fourth and fifth and enharmonically_equivalents.";
	tonality:semitones 5;
	.

int:ic6 a tonality:IntervalClass;
	rdfs:label "Interval class 6";
	vs:term_status "unstable";
	rdfs:comment "augmented fourth and diminished fifth and enharmonically_equivalents.";
	tonality:semitones 6;
	.

#####################Interval individuals################

int:unison a tonality:Interval;
	rdfs:label "unison";
	vs:term_status "unstable";
	rdfs:comment "Unison interval.";
	tonality:tuning tuning:twelve_edo;
	tonality:semitones 0;
	tonality:scale_steps 0;
	tonality:steps 0;
	tonality:cents 0;
	tonality:interval_class int:ic0;
	.

int:second_min a tonality:Interval;
	rdfs:label "minor 2nd";
	vs:term_status "unstable";
	rdfs:comment "Diatonic minor 2nd in 12 EDO.";
	tonality:tuning tuning:twelve_edo;
	tonality:scale_steps 1;
	tonality:semitones 1;
	tonality:steps 0.5;
	tonality:cents 100;
	tonality:interval_class int:ic1;
	dc:type "diatonic";
	.

int:second_maj a tonality:Interval;
	rdfs:label "major 2nd";
	vs:term_status "unstable";
	rdfs:comment "Diatonic major 2nd in 12 EDO.";
	tonality:tuning tuning:twelve_edo;
	tonality:scale_steps 1;
	tonality:semitones 2;
	tonality:steps 1;
	tonality:cents 200;
	tonality:interval_class int:ic2;
	dc:type "diatonic";
	.

int:third_min a tonality:Interval;
	rdfs:label "minor 3rd";
	vs:term_status "unstable";
	rdfs:comment "Diatonic minor 3rd in 12 EDO.";
	tonality:tuning tuning:twelve_edo;
	tonality:scale_steps 2;
	tonality:semitones 3;
	tonality:steps 1.5;
	tonality:cents 300;
	tonality:interval_class int:ic3;
	dc:type "diatonic";
	.

int:third_maj a tonality:Interval;
	rdfs:label "major 3rd";
	vs:term_status "unstable";
	rdfs:comment "Diatonic major 3rd in 12 EDO.";
	tonality:tuning tuning:twelve_edo;
	tonality:scale_steps 2;
	tonality:semitones 4;
	tonality:steps 2;
	tonality:cents 400;
	tonality:interval_class int:ic4;
	dc:type "diatonic";
	.

int:fourth_per a tonality:Interval;
	rdfs:label "perfect 4th";
	vs:term_status "unstable";
	rdfs:comment "Diatonic perfect fourth 12 EDO.";
	tonality:tuning tuning:twelve_edo;
	tonality:scale_steps 3;
	tonality:semitones 5;
	tonality:steps 2.5;
	tonality:cents 500;
	tonality:interval_class int:ic5;
	dc:type "diatonic";
	.

int:fourth_aug a tonality:Interval;
	rdfs:label "augmented 4th";
	vs:term_status "unstable";
	rdfs:comment "Chromatic augmented fourth 12 EDO.";
	tonality:tuning tuning:twelve_edo;
	tonality:scale_steps 3;
	tonality:semitones 6;
	tonality:steps 3;
	tonality:cents 600;
	tonality:interval_class int:ic6;
	dc:type "chromatic";
	.

int:fifth_dim a tonality:Interval;
	rdfs:label "diminished 5th";
	vs:term_status "unstable";
	rdfs:comment "Chromatic diminished 5th 12 EDO.";
	tonality:tuning tuning:twelve_edo;
	tonality:scale_steps 4;
	tonality:semitones 6;
	tonality:steps 3;
	tonality:cents 600;
	tonality:interval_class int:ic6;
	dc:type "chromatic";
	tonality:enharmonically_equivalent int:fourth_aug;
	tonality:inversion int:fourth_aug;
	.

int:fifth_per a tonality:Interval;
	rdfs:label "perfect fifth";
	vs:term_status "unstable";
	rdfs:comment "Diatonic perfect fifth in 12 EDO.";
	tonality:tuning tuning:twelve_edo;
	tonality:scale_steps 4;
	tonality:semitones 7;
	tonality:steps 3.5;
	tonality:cents 700;
	dc:type "diatonic";
	tonality:interval_class int:ic5;
	tonality:inversion int:fourth_per;
	.

int:sixth_min a tonality:Interval;
	rdfs:label "minor 6th";
	vs:term_status "unstable";
	rdfs:comment "Diatonic minor sixth in 12 EDO.";
	tonality:tuning tuning:twelve_edo;
	tonality:scale_steps 5;
	tonality:semitones 8;
	tonality:steps 4;
	tonality:cents 800;
	tonality:interval_class int:ic4;
	dc:type "diatonic";
	tonality:inversion int:third_maj;
	.

int:sixth_maj a tonality:Interval;
	rdfs:label "major 6th";
	vs:term_status "unstable";
	rdfs:comment "Diatonic major sixth in 12 EDO.";
	tonality:tuning tuning:twelve_edo;
	tonality:scale_steps 5;
	tonality:semitones 9;
	tonality:steps 4.5;
	tonality:cents 900;
	tonality:interval_class int:ic3;
	dc:type "diatonic";
	tonality:inversion int:third_min;
	.

int:seventh_min a tonality:Interval;
	rdfs:label "minor 7th";
	vs:term_status "unstable";
	rdfs:comment "Diatonic minor seventh in 12 EDO.";
	tonality:tuning tuning:twelve_edo;
	tonality:scale_steps 6;
	tonality:semitones 10;
	tonality:steps 5;
	tonality:cents 1000;
	tonality:interval_class int:ic2;
	dc:type "diatonic";
	tonality:inversion int:second_maj;
	.

int:seventh_maj a tonality:Interval;
	rdfs:label "major 7th";
	vs:term_status "unstable";
	rdfs:comment "Diatonic major seventh in 12 EDO.";
	tonality:tuning tuning:twelve_edo;
	tonality:scale_steps 6;
	tonality:semitones 11;
	tonality:steps 5.5;
	tonality:cents 1100;
	tonality:interval_class int:ic1;
	dc:type "diatonic";
	tonality:inversion int:second_min;
	.

int:octave a tonality:Interval;
	rdfs:label "octave";
	rdfs:comment "Octave.";
	vs:term_status "unstable";
	tonality:tuning tuning:twelve_edo;
	tonality:scale_steps 12;
	tonality:semitones 12;
	tonality:steps 6;
	tonality:cents 1200;
	tonality:interval_class int:ic0;
	dc:type "diatonic";
	.

#Example of compound interval

int:ninth_min a tonality:Interval;
	rdfs:label "minor 9th";
	vs:term_status "unstable";
	rdfs:comment "compound interval of a minor second in the next octave (12-EDO)";
	tonality:tuning tuning:twelve_edo;
	tonality:simple_interval int:second_min;
	tonality:octaves 1;
	.

int:tritone a tonality:Interval;
	rdfs:label "tritone";
	vs:term_status "unstable";
	rdfs:comment """
		Interval composed by 3 semitones in 12 EDO. Main interval of dissonance in Western music and really important in Harmony as it defines a the function of the dominant degree (which should be major with minor seventh).
	""";
	tonality:tuning tuning:twelve_edo;	
	tonality:interval_class int:ic6;
	tonality:semitones 6;
	tonality:steps 3;
	tonality:cents 600;
	tonality:strength "dissonant";
	tonality:enharmonically_equivalent int:fifth_dim;
	tonality:enharmonically_equivalent int:fourth_aug;
	.

#################### Mode Individuals ###############

mode:major a tonality:Mode;
	rdfs:label "major mode";
	vs:term_status "unstable";
	rdfs:comment "The major mode (ionian)";
	tonality:num_degrees 7;
	tonality:degree [ a tonality:Degree;
			tonality:degree_position 1;
			tonality:interval int:unison],	
			[ a tonality:Degree;
			tonality:degree_position 2;
			tonality:interval int:second_maj],
			[ a tonality:Degree;
			tonality:degree_position 3;
			tonality:interval int:third_maj],
			[ a tonality:Degree;
			tonality:degree_position 4;
			tonality:interval int:fourth_per],
			[ a tonality:Degree;
			tonality:degree_position 5;
			tonality:interval int:fifth_per],
			[ a tonality:Degree;
			tonality:degree_position 6;
			tonality:interval int:sixth_maj],
			[ a tonality:Degree;
			tonality:degree_position 7;
			tonality:interval int:seventh_maj];
	.

mode:minor a tonality:Mode;
	rdfs:label "Natural Minor mode";
	vs:term_status "unstable";
	rdfs:comment """
		The Natural Minor scale which is the minor relative of the major scale and the Eolian mode of the diatonic scale. It is a very stable scale but it lacks a major seventh
	""";
	tonality:num_degrees 7;
	tonality:degree [ a tonality:Degree;
			tonality:degree_position 1;
			tonality:interval int:unison],	
			[ a tonality:Degree;
			tonality:degree_position 2;
			tonality:interval int:second_maj],
			[ a tonality:Degree;
			tonality:degree_position 3;
			tonality:interval int:third_min],
			[ a tonality:Degree;
			tonality:degree_position 4;
			tonality:interval int:fourth_per],
			[ a tonality:Degree;
			tonality:degree_position 5;
			tonality:interval int:fifth_per],
			[ a tonality:Degree;
			tonality:degree_position 6;
			tonality:interval int:sixth_min],
			[ a tonality:Degree;
			tonality:degree_position 7;
			tonality:interval int:seventh_min];
	.

mode:harmonic_minor a tonality:Mode;
	rdfs:label "Harmonic Minor Mode";
	vs:term_status "unstable";
	rdfs:comment """
		The Harmonic Minor mode alters the seventh degree which is a major seventh and is a very used scale as it provides a dominant major with seventh minor. Often referred as a scale, but strictly we should talk as mode.
	""";
	tonality:num_degrees 7;
	tonality:degree [ a tonality:Degree;
			tonality:degree_position 1;
			tonality:interval int:unison],	
			[ a tonality:Degree;
			tonality:degree_position 2;
			tonality:interval int:second_maj],
			[ a tonality:Degree;
			tonality:degree_position 3;
			tonality:interval int:third_min],
			[ a tonality:Degree;
			tonality:degree_position 4;
			tonality:interval int:fourth_per],
			[ a tonality:Degree;
			tonality:degree_position 5;
			tonality:interval int:fifth_per],
			[ a tonality:Degree;
			tonality:degree_position 6;
			tonality:interval int:sixth_min],
			[ a tonality:Degree;
			tonality:degree_position 7;
			tonality:interval int:seventh_maj];
	.
	
mode:pentatonic_min a tonality:Mode;
	rdfs:label "Pentatonic minor mode";
	vs:term_status "unstable";
	rdfs:comment "Pentatonic minor mode.";
	tonality:num_degrees 5;
	tonality:degree [ a tonality:Degree;
			tonality:degree_position 1;
			tonality:interval int:unison],	
			[ a tonality:Degree;
			tonality:degree_position 2;
			tonality:interval int:third_min],
			[ a tonality:Degree;
			tonality:degree_position 3;
			tonality:interval int:fourth_per],
			[ a tonality:Degree;
			tonality:degree_position 4;
			tonality:interval int:fifth_per],
			[ a tonality:Degree;
			tonality:degree_position 6;
			tonality:interval int:seventh_min];
	.

mode:pentatonic_maj a tonality:Mode;
	rdfs:label "Pentatonic major mode";
	rdfs:comment "The Pentatonic major mode";
	vs:term_status "unstable";
	tonality:num_degrees 5;
	tonality:degree [ a tonality:Degree;
			tonality:degree_position 1;
			tonality:interval int:unison],	
			[ a tonality:Degree;
			tonality:degree_position 2;
			tonality:interval int:second_maj],
			[ a tonality:Degree;
			tonality:degree_position 3;
			tonality:interval int:third_maj],
			[ a tonality:Degree;
			tonality:degree_position 4;
			tonality:interval int:fifth_per],
			[ a tonality:Degree;
			tonality:degree_position 5;
			tonality:interval int:sixth_maj];
	.

scale:majorA
	a tonality:DiatonicScale;
	rdfs:label "A major scale";
	vs:term_status "unstable";
	rdfs:comment "Major scale in A (the minor mode starting in A)";
	tonality:mode mode:major;
	tonality:tonic note:A;
	.

###########Modes individuals ############ Problems to define what is minor...

mode:ionian
	a tonality:Mode;
	rdfs:label "Ionian mode";
	vs:term_status "unstable";
	rdfs:comment "First mode used over a diatonic set";
	owl:sameAs mode:major;
	.

mode:dorian
	a tonality:Mode;
	rdfs:label "Dorian mode";
	vs:term_status "unstable";
	rdfs:comment "Second mode of a diatonic set.";
	tonality:num_degrees 7;
	tonality:degree [ a tonality:Degree;
			tonality:degree_position 1;
			tonality:interval int:unison],	
			[ a tonality:Degree;
			tonality:degree_position 2;
			tonality:interval int:second_maj],
			[ a tonality:Degree;
			tonality:degree_position 3;
			tonality:interval int:third_min],
			[ a tonality:Degree;
			tonality:degree_position 4;
			tonality:interval int:fourth_per],
			[ a tonality:Degree;
			tonality:degree_position 5;
			tonality:interval int:fifth_per],
			[ a tonality:Degree;
			tonality:degree_position 6;
			tonality:interval int:sixth_maj],
			[ a tonality:Degree;
			tonality:degree_position 7;
			tonality:interval int:seventh_min];
	.

mode:phrygian
	a tonality:Mode;
	rdfs:label "Phrygian mode";
	vs:term_status "unstable";
	rdfs:comment "Third mode of a diatonic set.";
	tonality:num_degrees 7;
	tonality:degree [ a tonality:Degree;
			tonality:degree_position 1;
			tonality:interval int:unison],	
			[ a tonality:Degree;
			tonality:degree_position 2;
			tonality:interval int:second_min],
			[ a tonality:Degree;
			tonality:degree_position 3;
			tonality:interval int:third_min],
			[ a tonality:Degree;
			tonality:degree_position 4;
			tonality:interval int:fourth_per],
			[ a tonality:Degree;
			tonality:degree_position 5;
			tonality:interval int:fifth_per],
			[ a tonality:Degree;
			tonality:degree_position 6;
			tonality:interval int:sixth_min],
			[ a tonality:Degree;
			tonality:degree_position 7;
			tonality:interval int:seventh_min];
	.

mode:lydian
	a tonality:Mode;
	rdfs:label "Lydian mode";
	vs:term_status "unstable";
	rdfs:comment "Fourth mode of a diatonic set.";
	tonality:num_degrees 7;
	tonality:degree [ a tonality:Degree;
			tonality:degree_position 1;
			tonality:interval int:unison],	
			[ a tonality:Degree;
			tonality:degree_position 2;
			tonality:interval int:second_maj],
			[ a tonality:Degree;
			tonality:degree_position 3;
			tonality:interval int:third_maj],
			[ a tonality:Degree;
			tonality:degree_position 4;
			tonality:interval int:fourth_aug],
			[ a tonality:Degree;
			tonality:degree_position 5;
			tonality:interval int:fifth_per],
			[ a tonality:Degree;
			tonality:degree_position 6;
			tonality:interval int:sixth_maj],
			[ a tonality:Degree;
			tonality:degree_position 7;
			tonality:interval int:seventh_maj];
	.

mode:mixolydian
	a tonality:Mode;
	rdfs:label "Mixolydian mode";
	vs:term_status "unstable";
	rdfs:comment "Fifth mode of a diatonic scale.";
	tonality:num_degrees 7;
	tonality:degree [ a tonality:Degree;
			tonality:degree_position 1;
			tonality:interval int:unison],	
			[ a tonality:Degree;
			tonality:degree_position 2;
			tonality:interval int:second_maj],
			[ a tonality:Degree;
			tonality:degree_position 3;
			tonality:interval int:third_maj],
			[ a tonality:Degree;
			tonality:degree_position 4;
			tonality:interval int:fourth_per],
			[ a tonality:Degree;
			tonality:degree_position 5;
			tonality:interval int:fifth_per],
			[ a tonality:Degree;
			tonality:degree_position 6;
			tonality:interval int:sixth_maj],
			[ a tonality:Degree;
			tonality:degree_position 7;
			tonality:interval int:seventh_maj];
	.

mode:aeolian
	a tonality:Mode;
	rdfs:label "Aeolian mode";
	vs:term_status "unstable";
	rdfs:comment "Sixth mode of a diatonic scale (minor scale).";
	owl:sameAs mode:minor;
	.

mode:locrian
	a tonality:Mode;
	rdfs:label "Locrian mode";
	vs:term_status "unstable";
	rdfs:comment """
		Seventh mode of a diatonic scale. The main characteristic is the diminished fifth which makes this mode very intestable and used in Jazz for example.
	""";
	tonality:num_degrees 7;
	tonality:degree [ a tonality:Degree;
			tonality:degree_position 1;
			tonality:interval int:unison],	
			[ a tonality:Degree;
			tonality:degree_position 2;
			tonality:interval int:second_min],
			[ a tonality:Degree;
			tonality:degree_position 3;
			tonality:interval int:third_maj],
			[ a tonality:Degree;
			tonality:degree_position 4;
			tonality:interval int:fourth_per],
			[ a tonality:Degree;
			tonality:degree_position 5;
			tonality:interval int:fifth_dim],
			[ a tonality:Degree;
			tonality:degree_position 6;
			tonality:interval int:sixth_min],
			[ a tonality:Degree;
			tonality:degree_position 7;
			tonality:interval int:seventh_maj];
	.
	.

####################Keys individuals (12 EDO)######################

#C

key:Cmajor
	a tonality:Key;
	rdfs:label "C major key";
	vs:term_status "testing";
	rdfs:comment "Description of the C major key.";
	tonality:tonic note:C;
	tonality:degree [ a tonality:Degree;
			tonality:degree_position 1;
			tonality:degree_name "Tonic";
			tonality:note note:C;
			tonality:owned_chord co:maj7;
			tonality:interval int:unison],	
			[ a tonality:Degree;
			tonality:degree_position 2;
			tonality:degree_name "Supertonic";
			tonality:note note:D;
			tonality:owned_chord co:min7;
			tonality:interval int:second_maj],
			[ a tonality:Degree;
			tonality:degree_position 3;
			tonality:degree_name "Mediant";
			tonality:note note:E;
			tonality:owned_chord co:min7;
			tonality:interval int:third_maj],
			[ a tonality:Degree;
			tonality:degree_position 4;
			tonality:degree_name "Subdominant";
			tonality:note note:F;
			tonality:owned_chord co:maj7;
			tonality:interval int:fourth_per],
			[ a tonality:Degree;
			tonality:degree_position 5;
			tonality:degree_name "Dominant";
			tonality:note note:G;
			tonality:owned_chord co:seventh;
			tonality:interval int:fifth_per],
			[ a tonality:Degree;
			tonality:degree_position 6;
			tonality:degree_name "Submediant";
			tonality:note note:A;
			tonality:owned_chord co:min7;
			tonality:interval int:sixth_maj],
			[ a tonality:Degree;
			tonality:degree_position 7;
			tonality:degree_name "Subtonic or Leading Tone";
			tonality:note note:B;
			tonality:owned_chord co:hdim7;
			tonality:interval int:seventh_maj];
	.

key:Cminor
	a tonality:Key;
	rdfs:label "C minor key";
	vs:term_status "testing";
	rdfs:comment "Description of the C minor key.";
	tonality:tonic note:C;
	tonality:degree [ a tonality:Degree;
			tonality:degree_position 1;
			tonality:degree_name "Tonic";
			tonality:note note:C;
			tonality:owned_chord co:min7;
			tonality:interval int:unison],	
			[ a tonality:Degree;
			tonality:degree_position 2;
			tonality:degree_name "Supertonic";
			tonality:note note:D;
			tonality:owned_chord co:hdim7;
			tonality:interval int:second_maj],
			[ a tonality:Degree;
			tonality:degree_position 3;
			tonality:degree_name "Mediant";
			tonality:note note:Eb;
			tonality:owned_chord co:maj7;
			tonality:interval int:third_min],
			[ a tonality:Degree;
			tonality:degree_position 4;
			tonality:degree_name "Subdominant";
			rdfs:comment "This degree may appear altered borrowing the chord from the melodic minor scale.";
			tonality:note note:F;
			tonality:owned_chord co:min7;
			tonality:borrowed_chord co:seventh;
			tonality:interval int:fourth_per],
			[ a tonality:Degree;
			tonality:degree_position 5;
			tonality:degree_name "Dominant";
			rdfs:comment "This degree may appear altered borrowing the chord from the harmonic minor scale.";
			tonality:note note:G;
			tonality:owned_chord co:min7;
			tonality:borrowed_chord co:seventh;
			tonality:interval int:fifth_per],
			[ a tonality:Degree;
			tonality:degree_position 6;
			tonality:degree_name "Submediant";
			tonality:note note:Ab;
			tonality:owned_chord co:maj7;
			tonality:interval int:sixth_min],
			[ a tonality:Degree;
			tonality:degree_position 7;
			tonality:degree_name "Subtonic or Leading Tone";
			tonality:note note:Bb;
			tonality:owned_chord co:seventh;
			tonality:borrowed_chord co:dim7;
			tonality:interval int:seventh_min];
	.

#C sharp

key:Csmajor
	a tonality:Key;
	rdfs:label "C sharp major key";
	vs:term_status "testing";
	rdfs:comment "Description of the C sharp major key.";
	tonality:tonic note:Cs;
	tonality:degree [ a tonality:Degree;
			tonality:degree_position 1;
			tonality:degree_name "Tonic";
			tonality:note note:Cs;
			tonality:owned_chord co:maj7;
			tonality:interval int:unison],	
			[ a tonality:Degree;
			tonality:degree_position 2;
			tonality:degree_name "Supertonic";
			tonality:note note:Ds;
			tonality:owned_chord co:min7;
			tonality:interval int:second_maj],
			[ a tonality:Degree;
			tonality:degree_position 3;
			tonality:degree_name "Mediant";
			tonality:note note:Es;
			tonality:owned_chord co:min7;
			tonality:interval int:third_maj],
			[ a tonality:Degree;
			tonality:degree_position 4;
			tonality:degree_name "Subdominant";
			tonality:note note:Fs;
			tonality:owned_chord co:maj7;
			tonality:interval int:fourth_per],
			[ a tonality:Degree;
			tonality:degree_position 5;
			tonality:degree_name "Dominant";
			tonality:note note:Gs;
			tonality:owned_chord co:seventh;
			tonality:interval int:fifth_per],
			[ a tonality:Degree;
			tonality:degree_position 6;
			tonality:degree_name "Submediant";
			tonality:note note:As;
			tonality:owned_chord co:min7;
			tonality:interval int:sixth_maj],
			[ a tonality:Degree;
			tonality:degree_position 7;
			tonality:degree_name "Subtonic or Leading Tone";
			tonality:note note:Bs;
			tonality:owned_chord co:hdim7;
			tonality:interval int:seventh_maj];
	.

key:Csminor
	a tonality:Key;
	rdfs:label "C sharp minor key";
	vs:term_status "testing";
	rdfs:comment "Description of the C sharp minor key.";
	tonality:tonic note:Cs;
	tonality:degree [ a tonality:Degree;
			tonality:degree_position 1;
			tonality:degree_name "Tonic";
			tonality:note note:Cs;
			tonality:owned_chord co:min7;
			tonality:interval int:unison],	
			[ a tonality:Degree;
			tonality:degree_position 2;
			tonality:degree_name "Supertonic";
			tonality:note note:Ds;
			tonality:owned_chord co:hdim7;
			tonality:interval int:second_maj],
			[ a tonality:Degree;
			tonality:degree_position 3;
			tonality:degree_name "Mediant";
			tonality:note note:E;
			tonality:owned_chord co:maj7;
			tonality:interval int:third_min],
			[ a tonality:Degree;
			tonality:degree_position 4;
			tonality:degree_name "Subdominant";
			rdfs:comment "This degree may appear altered borrowing the chord from the melodic minor scale.";
			tonality:note note:Fs;
			tonality:owned_chord co:min7;
			tonality:borrowed_chord co:seventh;
			tonality:interval int:fourth_per],
			[ a tonality:Degree;
			tonality:degree_position 5;
			tonality:degree_name "Dominant";
			rdfs:comment "This degree may appear altered borrowing the chord from the harmonic minor scale.";
			tonality:note note:G;
			tonality:owned_chord co:min7;
			tonality:borrowed_chord co:seventh;
			tonality:interval int:fifth_per],
			[ a tonality:Degree;
			tonality:degree_position 6;
			tonality:degree_name "Submediant";
			tonality:note note:A;
			tonality:owned_chord co:maj7;
			tonality:interval int:sixth_min],
			[ a tonality:Degree;
			tonality:degree_position 7;
			tonality:degree_name "Subtonic or Leading Tone";
			tonality:note note:B;
			tonality:owned_chord co:seventh;
			tonality:borrowed_chord co:dim7;
			tonality:interval int:seventh_min];
	.

#D flat

key:Dbmajor
	a tonality:Key;
	rdfs:label "D flat major key";
	vs:term_status "testing";
	rdfs:comment "Description of the D  flat major key.";
	tonality:tonic note:Db;
	owl:sameAs key:Csmajor;
	.

key:Dbminor
	a tonality:Key;
	rdfs:label "D flat minor key";
	vs:term_status "testing";
	rdfs:comment "Description of the D  flat minor key.";
	tonality:tonic note:Db;
	owl:sameAs key:Csminor;
	.

#D

key:Dmajor
	a tonality:Key;
	rdfs:label "D major key";
	vs:term_status "testing";
	rdfs:comment "Description of the D major key.";
	tonality:tonic note:D;
	tonality:degree [ a tonality:Degree;
			tonality:degree_position 1;
			tonality:degree_name "Tonic";
			tonality:note note:D;
			tonality:owned_chord co:maj7;
			tonality:interval int:unison],	
			[ a tonality:Degree;
			tonality:degree_position 2;
			tonality:degree_name "Supertonic";
			tonality:note note:E;
			tonality:owned_chord co:min7;
			tonality:interval int:second_maj],
			[ a tonality:Degree;
			tonality:degree_position 3;
			tonality:degree_name "Mediant";
			tonality:note note:Fs;
			tonality:owned_chord co:min7;
			tonality:interval int:third_maj],
			[ a tonality:Degree;
			tonality:degree_position 4;
			tonality:degree_name "Subdominant";
			tonality:note note:G;
			tonality:owned_chord co:maj7;
			tonality:interval int:fourth_per],
			[ a tonality:Degree;
			tonality:degree_position 5;
			tonality:degree_name "Dominant";
			tonality:note note:A;
			tonality:owned_chord co:seventh;
			tonality:interval int:fifth_per],
			[ a tonality:Degree;
			tonality:degree_position 6;
			tonality:degree_name "Submediant";
			tonality:note note:B;
			tonality:owned_chord co:min7;
			tonality:interval int:sixth_maj],
			[ a tonality:Degree;
			tonality:degree_position 7;
			tonality:degree_name "Subtonic or Leading Tone";
			tonality:note note:Cs;
			tonality:owned_chord co:hdim7;
			tonality:interval int:seventh_maj];
	.

key:Dminor
	a tonality:Key;
	rdfs:label "D minor key";
	vs:term_status "testing";
	rdfs:comment "Description of the D minor key.";
	tonality:tonic note:D;
	tonality:degree [ a tonality:Degree;
			tonality:degree_position 1;
			tonality:degree_name "Tonic";
			tonality:note note:D;
			tonality:owned_chord co:min7;
			tonality:interval int:unison],	
			[ a tonality:Degree;
			tonality:degree_position 2;
			tonality:degree_name "Supertonic";
			tonality:note note:E;
			tonality:owned_chord co:hdim7;
			tonality:interval int:second_maj],
			[ a tonality:Degree;
			tonality:degree_position 3;
			tonality:degree_name "Mediant";
			tonality:note note:F;
			tonality:owned_chord co:maj7;
			tonality:interval int:third_min],
			[ a tonality:Degree;
			tonality:degree_position 4;
			tonality:degree_name "Subdominant";
			rdfs:comment "This degree may appear altered borrowing the chord from the melodic minor scale.";
			tonality:note note:G;
			tonality:owned_chord co:min7;
			tonality:borrowed_chord co:seventh;
			tonality:interval int:fourth_per],
			[ a tonality:Degree;
			tonality:degree_position 5;
			tonality:degree_name "Dominant";
			rdfs:comment "This degree may appear altered borrowing the chord from the harmonic minor scale.";
			tonality:note note:A;
			tonality:owned_chord co:min7;
			tonality:borrowed_chord co:seventh;
			tonality:interval int:fifth_per],
			[ a tonality:Degree;
			tonality:degree_position 6;
			tonality:degree_name "Submediant";
			tonality:note note:Bb;
			tonality:owned_chord co:maj7;
			tonality:interval int:sixth_min],
			[ a tonality:Degree;
			tonality:degree_position 7;
			tonality:degree_name "Subtonic or Leading Tone";
			tonality:note note:C;
			tonality:owned_chord co:seventh;
			tonality:borrowed_chord co:dim7;
			tonality:interval int:seventh_min];
	.

#D Sharp

key:Dsmajor
	a tonality:Key;
	rdfs:label "D sharp major key";
	vs:term_status "testing";
	rdfs:comment "Description of the D sharp major key.";
	tonality:tonic note:Ds;
	tonality:degree [ a tonality:Degree;
			tonality:degree_position 1;
			tonality:degree_name "Tonic";
			tonality:note note:Ds;
			tonality:owned_chord co:maj7;
			tonality:interval int:unison],	
			[ a tonality:Degree;
			tonality:degree_position 2;
			tonality:degree_name "Supertonic";
			tonality:note note:F;
			tonality:owned_chord co:min7;
			tonality:interval int:second_maj],
			[ a tonality:Degree;
			tonality:degree_position 3;
			tonality:degree_name "Mediant";
			tonality:note note:G;
			tonality:owned_chord co:min7;
			tonality:interval int:third_maj],
			[ a tonality:Degree;
			tonality:degree_position 4;
			tonality:degree_name "Subdominant";
			tonality:note note:Gs;
			tonality:owned_chord co:maj7;
			tonality:interval int:fourth_per],
			[ a tonality:Degree;
			tonality:degree_position 5;
			tonality:degree_name "Dominant";
			tonality:note note:As;
			tonality:owned_chord co:seventh;
			tonality:interval int:fifth_per],
			[ a tonality:Degree;
			tonality:degree_position 6;
			tonality:degree_name "Submediant";
			tonality:note note:C;
			tonality:owned_chord co:min7;
			tonality:interval int:sixth_maj],
			[ a tonality:Degree;
			tonality:degree_position 7;
			tonality:degree_name "Subtonic or Leading Tone";
			tonality:note note:D;
			tonality:owned_chord co:hdim7;
			tonality:interval int:seventh_maj];
	.

key:Dsminor
	a tonality:Key;
	rdfs:label "D sharp minor key";
	vs:term_status "testing";
	rdfs:comment "Description of the D sharp minor key.";
	tonality:tonic note:Ds;
	tonality:degree [ a tonality:Degree;
			tonality:degree_position 1;
			tonality:degree_name "Tonic";
			tonality:note note:Ds;
			tonality:owned_chord co:min7;
			tonality:interval int:unison],	
			[ a tonality:Degree;
			tonality:degree_position 2;
			tonality:degree_name "Supertonic";
			tonality:note note:F;
			tonality:owned_chord co:hdim7;
			tonality:interval int:second_maj],
			[ a tonality:Degree;
			tonality:degree_position 3;
			tonality:degree_name "Mediant";
			tonality:note note:Fs;
			tonality:owned_chord co:maj7;
			tonality:interval int:third_min],
			[ a tonality:Degree;
			tonality:degree_position 4;
			tonality:degree_name "Subdominant";
			rdfs:comment "This degree may appear altered borrowing the chord from the melodic minor scale.";
			tonality:note note:Gs;
			tonality:owned_chord co:min7;
			tonality:borrowed_chord co:seventh;
			tonality:interval int:fourth_per],
			[ a tonality:Degree;
			tonality:degree_position 5;
			tonality:degree_name "Dominant";
			rdfs:comment "This degree may appear altered borrowing the chord from the harmonic minor scale.";
			tonality:note note:As;
			tonality:owned_chord co:min7;
			tonality:borrowed_chord co:seventh;
			tonality:interval int:fifth_per],
			[ a tonality:Degree;
			tonality:degree_position 6;
			tonality:degree_name "Submediant";
			tonality:note note:B;
			tonality:owned_chord co:maj7;
			tonality:interval int:sixth_min],
			[ a tonality:Degree;
			tonality:degree_position 7;
			tonality:degree_name "Subtonic or Leading Tone";
			tonality:note note:Cs;
			tonality:owned_chord co:seventh;
			tonality:borrowed_chord co:dim7;
			tonality:interval int:seventh_min];
	.

#E flat

key:Ebmajor
	a tonality:Key;
	rdfs:label "E flat major key";
	vs:term_status "testing";
	rdfs:comment "Description of the E flat major key.";
	tonality:tonic note:Eb;
	owl:sameAs key:Dsmajor;
	.

key:Ebminor
	a tonality:Key;
	rdfs:label "E flat minor key";
	vs:term_status "testing";
	rdfs:comment "Description of the E flat minor key.";
	tonality:tonic note:Eb;
	owl:sameAs key:Dsminor;
	.

#E

key:Emajor
	a tonality:Key;
	rdfs:label "E major key";
	vs:term_status "testing";
	rdfs:comment "Description of the E major key.";
	tonality:tonic note:E;
	tonality:degree [ a tonality:Degree;
			tonality:degree_position 1;
			tonality:degree_name "Tonic";
			tonality:note note:E;
			tonality:owned_chord co:maj7;
			tonality:interval int:unison],	
			[ a tonality:Degree;
			tonality:degree_position 2;
			tonality:degree_name "Supertonic";
			tonality:note note:Fs;
			tonality:owned_chord co:min7;
			tonality:interval int:second_maj],
			[ a tonality:Degree;
			tonality:degree_position 3;
			tonality:degree_name "Mediant";
			tonality:note note:Gs;
			tonality:owned_chord co:min7;
			tonality:interval int:third_maj],
			[ a tonality:Degree;
			tonality:degree_position 4;
			tonality:degree_name "Subdominant";
			tonality:note note:A;
			tonality:owned_chord co:maj7;
			tonality:interval int:fourth_per],
			[ a tonality:Degree;
			tonality:degree_position 5;
			tonality:degree_name "Dominant";
			tonality:note note:B;
			tonality:owned_chord co:seventh;
			tonality:interval int:fifth_per],
			[ a tonality:Degree;
			tonality:degree_position 6;
			tonality:degree_name "Submediant";
			tonality:note note:Cs;
			tonality:owned_chord co:min7;
			tonality:interval int:sixth_maj],
			[ a tonality:Degree;
			tonality:degree_position 7;
			tonality:degree_name "Subtonic or Leading Tone";
			tonality:note note:Ds;
			tonality:owned_chord co:hdim7;
			tonality:interval int:seventh_maj];
	.

key:Eminor
	a tonality:Key;
	rdfs:label "E minor key";
	vs:term_status "testing";
	rdfs:comment "Description of the E minor key.";
	tonality:tonic note:E;
	tonality:degree [ a tonality:Degree;
			tonality:degree_position 1;
			tonality:degree_name "Tonic";
			tonality:note note:E;
			tonality:owned_chord co:min7;
			tonality:interval int:unison],	
			[ a tonality:Degree;
			tonality:degree_position 2;
			tonality:degree_name "Supertonic";
			tonality:note note:Fs;
			tonality:owned_chord co:hdim7;
			tonality:interval int:second_maj],
			[ a tonality:Degree;
			tonality:degree_position 3;
			tonality:degree_name "Mediant";
			tonality:note note:G;
			tonality:owned_chord co:maj7;
			tonality:interval int:third_min],
			[ a tonality:Degree;
			tonality:degree_position 4;
			tonality:degree_name "Subdominant";
			rdfs:comment "This degree may appear altered borrowing the chord from the melodic minor scale.";
			tonality:note note:A;
			tonality:owned_chord co:min7;
			tonality:borrowed_chord co:seventh;
			tonality:interval int:fourth_per],
			[ a tonality:Degree;
			tonality:degree_position 5;
			tonality:degree_name "Dominant";
			rdfs:comment "This degree may appear altered borrowing the chord from the harmonic minor scale.";
			tonality:note note:B;
			tonality:owned_chord co:min7;
			tonality:borrowed_chord co:seventh;
			tonality:interval int:fifth_per],
			[ a tonality:Degree;
			tonality:degree_position 6;
			tonality:degree_name "Submediant";
			tonality:note note:C;
			tonality:owned_chord co:maj7;
			tonality:interval int:sixth_min],
			[ a tonality:Degree;
			tonality:degree_position 7;
			tonality:degree_name "Subtonic or Leading Tone";
			tonality:note note:D;
			tonality:owned_chord co:seventh;
			tonality:borrowed_chord co:dim7;
			tonality:interval int:seventh_min];
	.

#E SHARP

key:Esmajor
	a tonality:Key;
	rdfs:label "E sharp major key";
	vs:term_status "testing";
	rdfs:comment "Description of the E sharp major key.";
	tonality:tonic note:Es;
	owl:sameAs key:Fmajor;
	.

key:Esminor
	a tonality:Key;
	rdfs:label "E flat minor key";
	vs:term_status "testing";
	rdfs:comment "Description of the E flat minor key.";
	tonality:tonic note:Eb;
	owl:sameAs key:Dsminor;
	.


#F

key:Fmajor
	a tonality:Key;
	rdfs:label "F major key";
	vs:term_status "testing";
	rdfs:comment "Description of the F major key.";
	tonality:tonic note:F;
	tonality:degree [ a tonality:Degree;
			tonality:degree_position 1;
			tonality:degree_name "Tonic";
			tonality:note note:F;
			tonality:owned_chord co:maj7;
			tonality:interval int:unison],	
			[ a tonality:Degree;
			tonality:degree_position 2;
			tonality:degree_name "Supertonic";
			tonality:note note:G;
			tonality:owned_chord co:min7;
			tonality:interval int:second_maj],
			[ a tonality:Degree;
			tonality:degree_position 3;
			tonality:degree_name "Mediant";
			tonality:note note:A;
			tonality:owned_chord co:min7;
			tonality:interval int:third_maj],
			[ a tonality:Degree;
			tonality:degree_position 4;
			tonality:degree_name "Subdominant";
			tonality:note note:Bb;
			tonality:owned_chord co:maj7;
			tonality:interval int:fourth_per],
			[ a tonality:Degree;
			tonality:degree_position 5;
			tonality:degree_name "Dominant";
			tonality:note note:C;
			tonality:owned_chord co:seventh;
			tonality:interval int:fifth_per],
			[ a tonality:Degree;
			tonality:degree_position 6;
			tonality:degree_name "Submediant";
			tonality:note note:D;
			tonality:owned_chord co:min7;
			tonality:interval int:sixth_maj],
			[ a tonality:Degree;
			tonality:degree_position 7;
			tonality:degree_name "Subtonic or Leading Tone";
			tonality:note note:E;
			tonality:owned_chord co:hdim7;
			tonality:interval int:seventh_maj];
	.

key:Fminor
	a tonality:Key;
	rdfs:label "F minor key";
	vs:term_status "testing";
	rdfs:comment "Description of the F minor key.";
	tonality:tonic note:F;
	tonality:degree [ a tonality:Degree;
			tonality:degree_position 1;
			tonality:degree_name "Tonic";
			tonality:note note:F;
			tonality:owned_chord co:min7;
			tonality:interval int:unison],	
			[ a tonality:Degree;
			tonality:degree_position 2;
			tonality:degree_name "Supertonic";
			tonality:note note:G;
			tonality:owned_chord co:hdim7;
			tonality:interval int:second_maj],
			[ a tonality:Degree;
			tonality:degree_position 3;
			tonality:degree_name "Mediant";
			tonality:note note:Ab;
			tonality:owned_chord co:maj7;
			tonality:interval int:third_min],
			[ a tonality:Degree;
			tonality:degree_position 4;
			tonality:degree_name "Subdominant";
			rdfs:comment "This degree may appear altered borrowing the chord from the melodic minor scale.";
			tonality:note note:Bb;
			tonality:owned_chord co:min7;
			tonality:borrowed_chord co:seventh;
			tonality:interval int:fourth_per],
			[ a tonality:Degree;
			tonality:degree_position 5;
			tonality:degree_name "Dominant";
			rdfs:comment "This degree may appear altered borrowing the chord from the harmonic minor scale.";
			tonality:note note:C;
			tonality:owned_chord co:min7;
			tonality:borrowed_chord co:seventh;
			tonality:interval int:fifth_per],
			[ a tonality:Degree;
			tonality:degree_position 6;
			tonality:degree_name "Submediant";
			tonality:note note:Db;
			tonality:owned_chord co:maj7;
			tonality:interval int:sixth_min],
			[ a tonality:Degree;
			tonality:degree_position 7;
			tonality:degree_name "Subtonic or Leading Tone";
			tonality:note note:Eb;
			tonality:owned_chord co:seventh;
			tonality:borrowed_chord co:dim7;
			tonality:interval int:seventh_min];
	.

#F sharp

key:Fsmajor
	a tonality:Key;
	rdfs:label "F sharp major key";
	vs:term_status "testing";
	rdfs:comment "Description of the F sharp major key.";
	tonality:tonic note:Fs;
	tonality:degree [ a tonality:Degree;
			tonality:degree_position 1;
			tonality:degree_name "Tonic";
			tonality:note note:Fs;
			tonality:owned_chord co:maj7;
			tonality:interval int:unison],	
			[ a tonality:Degree;
			tonality:degree_position 2;
			tonality:degree_name "Supertonic";
			tonality:note note:Gs;
			tonality:owned_chord co:min7;
			tonality:interval int:second_maj],
			[ a tonality:Degree;
			tonality:degree_position 3;
			tonality:degree_name "Mediant";
			tonality:note note:As;
			tonality:owned_chord co:min7;
			tonality:interval int:third_maj],
			[ a tonality:Degree;
			tonality:degree_position 4;
			tonality:degree_name "Subdominant";
			tonality:note note:B;
			tonality:owned_chord co:maj7;
			tonality:interval int:fourth_per],
			[ a tonality:Degree;
			tonality:degree_position 5;
			tonality:degree_name "Dominant";
			tonality:note note:Cs;
			tonality:owned_chord co:seventh;
			tonality:interval int:fifth_per],
			[ a tonality:Degree;
			tonality:degree_position 6;
			tonality:degree_name "Submediant";
			tonality:note note:Ds;
			tonality:owned_chord co:min7;
			tonality:interval int:sixth_maj],
			[ a tonality:Degree;
			tonality:degree_position 7;
			tonality:degree_name "Subtonic or Leading Tone";
			tonality:note note:Es;
			tonality:owned_chord co:hdim7;
			tonality:interval int:seventh_maj];
	.

key:Fsminor
	a tonality:Key;
	rdfs:label "F sharp minor key";
	vs:term_status "testing";
	rdfs:comment "Description of the F sharp minor key.";
	tonality:tonic note:Fs;
	tonality:degree [ a tonality:Degree;
			tonality:degree_position 1;
			tonality:degree_name "Tonic";
			tonality:note note:Fs;
			tonality:owned_chord co:min7;
			tonality:interval int:unison],	
			[ a tonality:Degree;
			tonality:degree_position 2;
			tonality:degree_name "Supertonic";
			tonality:note note:Gs;
			tonality:owned_chord co:hdim7;
			tonality:interval int:second_maj],
			[ a tonality:Degree;
			tonality:degree_position 3;
			tonality:degree_name "Mediant";
			tonality:note note:A;
			tonality:owned_chord co:maj7;
			tonality:interval int:third_min],
			[ a tonality:Degree;
			tonality:degree_position 4;
			tonality:degree_name "Subdominant";
			rdfs:comment "This degree may appear altered borrowing the chord from the melodic minor scale.";
			tonality:note note:B;
			tonality:owned_chord co:min7;
			tonality:borrowed_chord co:seventh;
			tonality:interval int:fourth_per],
			[ a tonality:Degree;
			tonality:degree_position 5;
			tonality:degree_name "Dominant";
			rdfs:comment "This degree may appear altered borrowing the chord from the harmonic minor scale.";
			tonality:note note:Cs;
			tonality:owned_chord co:min7;
			tonality:borrowed_chord co:seventh;
			tonality:interval int:fifth_per],
			[ a tonality:Degree;
			tonality:degree_position 6;
			tonality:degree_name "Submediant";
			tonality:note note:D;
			tonality:owned_chord co:maj7;
			tonality:interval int:sixth_min],
			[ a tonality:Degree;
			tonality:degree_position 7;
			tonality:degree_name "Subtonic or Leading Tone";
			tonality:note note:E;
			tonality:owned_chord co:seventh;
			tonality:borrowed_chord co:dim7;
			tonality:interval int:seventh_min];
	.

#G flat

key:Gbmajor
	a tonality:Key;
	rdfs:label "G flat major key";
	vs:term_status "testing";
	rdfs:comment "Description of the G flat major key.";
	tonality:tonic note:Gb;
	owl:sameAs key:Fsmajor;
	.

key:Gbminor
	a tonality:Key;
	rdfs:label "G flat minor key";
	vs:term_status "testing";
	rdfs:comment "Description of the G flat minor key.";
	tonality:tonic note:Gb;
	owl:sameAs key:Fsminor;
	.

#G

key:Gmajor
	a tonality:Key;
	rdfs:label "G major key";
	vs:term_status "testing";
	rdfs:comment "Description of the G major key.";
	tonality:tonic note:G;
	tonality:degree [ a tonality:Degree;
			tonality:degree_position 1;
			tonality:degree_name "Tonic";
			tonality:note note:G;
			tonality:owned_chord co:maj7;
			tonality:interval int:unison],	
			[ a tonality:Degree;
			tonality:degree_position 2;
			tonality:degree_name "Supertonic";
			tonality:note note:A;
			tonality:owned_chord co:min7;
			tonality:interval int:second_maj],
			[ a tonality:Degree;
			tonality:degree_position 3;
			tonality:degree_name "Mediant";
			tonality:note note:B;
			tonality:owned_chord co:min7;
			tonality:interval int:third_maj],
			[ a tonality:Degree;
			tonality:degree_position 4;
			tonality:degree_name "Subdominant";
			tonality:note note:C;
			tonality:owned_chord co:maj7;
			tonality:interval int:fourth_per],
			[ a tonality:Degree;
			tonality:degree_position 5;
			tonality:degree_name "Dominant";
			tonality:note note:D;
			tonality:owned_chord co:seventh;
			tonality:interval int:fifth_per],
			[ a tonality:Degree;
			tonality:degree_position 6;
			tonality:degree_name "Submediant";
			tonality:note note:E;
			tonality:owned_chord co:min7;
			tonality:interval int:sixth_maj],
			[ a tonality:Degree;
			tonality:degree_position 7;
			tonality:degree_name "Subtonic or Leading Tone";
			tonality:note note:Fs;
			tonality:owned_chord co:hdim7;
			tonality:interval int:seventh_maj];
	.

key:Gminor
	a tonality:Key;
	rdfs:label "G minor key";
	vs:term_status "testing";
	rdfs:comment "Description of the G minor key.";
	tonality:tonic note:G;
	tonality:degree [ a tonality:Degree;
			tonality:degree_position 1;
			tonality:degree_name "Tonic";
			tonality:note note:G;
			tonality:owned_chord co:min7;
			tonality:interval int:unison],	
			[ a tonality:Degree;
			tonality:degree_position 2;
			tonality:degree_name "Supertonic";
			tonality:note note:A;
			tonality:owned_chord co:hdim7;
			tonality:interval int:second_maj],
			[ a tonality:Degree;
			tonality:degree_position 3;
			tonality:degree_name "Mediant";
			tonality:note note:Bb;
			tonality:owned_chord co:maj7;
			tonality:interval int:third_min],
			[ a tonality:Degree;
			tonality:degree_position 4;
			tonality:degree_name "Subdominant";
			rdfs:comment "This degree may appear altered borrowing the chord from the melodic minor scale.";
			tonality:note note:C;
			tonality:owned_chord co:min7;
			tonality:borrowed_chord co:seventh;
			tonality:interval int:fourth_per],
			[ a tonality:Degree;
			tonality:degree_position 5;
			tonality:degree_name "Dominant";
			rdfs:comment "This degree may appear altered borrowing the chord from the harmonic minor scale.";
			tonality:note note:D;
			tonality:owned_chord co:min7;
			tonality:borrowed_chord co:seventh;
			tonality:interval int:fifth_per],
			[ a tonality:Degree;
			tonality:degree_position 6;
			tonality:degree_name "Submediant";
			tonality:note note:Eb;
			tonality:owned_chord co:maj7;
			tonality:interval int:sixth_min],
			[ a tonality:Degree;
			tonality:degree_position 7;
			tonality:degree_name "Subtonic or Leading Tone";
			tonality:note note:F;
			tonality:owned_chord co:seventh;
			tonality:borrowed_chord co:dim7;
			tonality:interval int:seventh_min];
	.

#G SHARP

key:Gsmajor
	a tonality:Key;
	rdfs:label "G sharp major key";
	vs:term_status "testing";
	rdfs:comment "Description of the G sharp major key.";
	tonality:tonic note:Gs;
	tonality:degree [ a tonality:Degree;
			tonality:degree_position 1;
			tonality:degree_name "Tonic";
			tonality:note note:Gs;
			tonality:owned_chord co:maj7;
			tonality:interval int:unison],	
			[ a tonality:Degree;
			tonality:degree_position 2;
			tonality:degree_name "Supertonic";
			tonality:note note:As;
			tonality:owned_chord co:min7;
			tonality:interval int:second_maj],
			[ a tonality:Degree;
			tonality:degree_position 3;
			tonality:degree_name "Mediant";
			tonality:note note:C;
			tonality:owned_chord co:min7;
			tonality:interval int:third_maj],
			[ a tonality:Degree;
			tonality:degree_position 4;
			tonality:degree_name "Subdominant";
			tonality:note note:Db;
			tonality:owned_chord co:maj7;
			tonality:interval int:fourth_per],
			[ a tonality:Degree;
			tonality:degree_position 5;
			tonality:degree_name "Dominant";
			tonality:note note:Eb;
			tonality:owned_chord co:seventh;
			tonality:interval int:fifth_per],
			[ a tonality:Degree;
			tonality:degree_position 6;
			tonality:degree_name "Submediant";
			tonality:note note:F;
			tonality:owned_chord co:min7;
			tonality:interval int:sixth_maj],
			[ a tonality:Degree;
			tonality:degree_position 7;
			tonality:degree_name "Subtonic or Leading Tone";
			tonality:note note:G;
			tonality:owned_chord co:hdim7;
			tonality:interval int:seventh_maj];
	.

key:Gsminor
	a tonality:Key;
	rdfs:label "G sharp minor key";
	vs:term_status "testing";
	rdfs:comment "Description of the G sharp minor key.";
	tonality:tonic note:Gs;
	tonality:degree [ a tonality:Degree;
			tonality:degree_position 1;
			tonality:degree_name "Tonic";
			tonality:note note:Gs;
			tonality:owned_chord co:min7;
			tonality:interval int:unison],	
			[ a tonality:Degree;
			tonality:degree_position 2;
			tonality:degree_name "Supertonic";
			tonality:note note:As;
			tonality:owned_chord co:hdim7;
			tonality:interval int:second_maj],
			[ a tonality:Degree;
			tonality:degree_position 3;
			tonality:degree_name "Mediant";
			tonality:note note:B;
			tonality:owned_chord co:maj7;
			tonality:interval int:third_min],
			[ a tonality:Degree;
			tonality:degree_position 4;
			tonality:degree_name "Subdominant";
			rdfs:comment "This degree may appear altered borrowing the chord from the melodic minor scale.";
			tonality:note note:Cs;
			tonality:owned_chord co:min7;
			tonality:borrowed_chord co:seventh;
			tonality:interval int:fourth_per],
			[ a tonality:Degree;
			tonality:degree_position 5;
			tonality:degree_name "Dominant";
			rdfs:comment "This degree may appear altered borrowing the chord from the harmonic minor scale.";
			tonality:note note:Ds;
			tonality:owned_chord co:min7;
			tonality:borrowed_chord co:seventh;
			tonality:interval int:fifth_per],
			[ a tonality:Degree;
			tonality:degree_position 6;
			tonality:degree_name "Submediant";
			tonality:note note:E;
			tonality:owned_chord co:maj7;
			tonality:interval int:sixth_min],
			[ a tonality:Degree;
			tonality:degree_position 7;
			tonality:degree_name "Subtonic or Leading Tone";
			tonality:note note:Fs;
			tonality:owned_chord co:seventh;
			tonality:borrowed_chord co:dim7;
			tonality:interval int:seventh_min];
	.

#A flat

key:Abmajor
	a tonality:Key;
	rdfs:label "A flat major key";
	vs:term_status "testing";
	rdfs:comment "Description of the A flat major key.";
	tonality:tonic note:Ab;
	owl:sameAs key:Gsmajor;
	.

key:Abminor
	a tonality:Key;
	rdfs:label "A flat minor key";
	vs:term_status "testing";
	rdfs:comment "Description of the A flat minor key.";
	tonality:tonic note:Ab;
	owl:sameAs key:Gsminor;
	.

#A

key:Amajor
	a tonality:Key;
	rdfs:label "A major key";
	vs:term_status "testing";
	rdfs:comment "Description of the A major key.";
	tonality:tonic note:A;
	tonality:degree [ a tonality:Degree;
			tonality:degree_position 1;
			tonality:degree_name "Tonic";
			tonality:note note:A;
			tonality:owned_chord co:maj7;
			tonality:interval int:unison],	
			[ a tonality:Degree;
			tonality:degree_position 2;
			tonality:degree_name "Supertonic";
			tonality:note note:B;
			tonality:owned_chord co:min7;
			tonality:interval int:second_maj],
			[ a tonality:Degree;
			tonality:degree_position 3;
			tonality:degree_name "Mediant";
			tonality:note note:Cs;
			tonality:owned_chord co:min7;
			tonality:interval int:third_maj],
			[ a tonality:Degree;
			tonality:degree_position 4;
			tonality:degree_name "Subdominant";
			tonality:note note:D;
			tonality:owned_chord co:maj7;
			tonality:interval int:fourth_per],
			[ a tonality:Degree;
			tonality:degree_position 5;
			tonality:degree_name "Dominant";
			tonality:note note:E;
			tonality:owned_chord co:seventh;
			tonality:interval int:fifth_per],
			[ a tonality:Degree;
			tonality:degree_position 6;
			tonality:degree_name "Submediant";
			tonality:note note:Fs;
			tonality:owned_chord co:min7;
			tonality:interval int:sixth_maj],
			[ a tonality:Degree;
			tonality:degree_position 7;
			tonality:degree_name "Subtonic or Leading Tone";
			tonality:note note:Ds;
			tonality:owned_chord co:hdim7;
			tonality:interval int:seventh_maj];
	.

key:Aminor
	a tonality:Key;
	rdfs:label "A minor key";
	vs:term_status "testing";
	rdfs:comment "Description of the A minor key.";
	tonality:tonic note:A;
	tonality:degree [ a tonality:Degree;
			tonality:degree_position 1;
			tonality:degree_name "Tonic";
			tonality:note note:A;
			tonality:owned_chord co:min7;
			tonality:interval int:unison],	
			[ a tonality:Degree;
			tonality:degree_position 2;
			tonality:degree_name "Supertonic";
			tonality:note note:B;
			tonality:owned_chord co:hdim7;
			tonality:interval int:second_maj],
			[ a tonality:Degree;
			tonality:degree_position 3;
			tonality:degree_name "Mediant";
			tonality:note note:C;
			tonality:owned_chord co:maj7;
			tonality:interval int:third_min],
			[ a tonality:Degree;
			tonality:degree_position 4;
			tonality:degree_name "Subdominant";
			rdfs:comment "This degree may appear altered borrowing the chord from the melodic minor scale.";
			tonality:note note:D;
			tonality:owned_chord co:min7;
			tonality:borrowed_chord co:seventh;
			tonality:interval int:fourth_per],
			[ a tonality:Degree;
			tonality:degree_position 5;
			tonality:degree_name "Dominant";
			rdfs:comment "This degree may appear altered borrowing the chord from the harmonic minor scale.";
			tonality:note note:E;
			tonality:owned_chord co:min7;
			tonality:borrowed_chord co:seventh;
			tonality:interval int:fifth_per],
			[ a tonality:Degree;
			tonality:degree_position 6;
			tonality:degree_name "Submediant";
			tonality:note note:F;
			tonality:owned_chord co:maj7;
			tonality:interval int:sixth_min],
			[ a tonality:Degree;
			tonality:degree_position 7;
			tonality:degree_name "Subtonic or Leading Tone";
			tonality:note note:G;
			tonality:owned_chord co:seventh;
			tonality:borrowed_chord co:dim7;
			tonality:interval int:seventh_min];
	.

#A SHARP 

key:Asmajor
	a tonality:Key;
	rdfs:label "A sharp major key";
	vs:term_status "testing";
	rdfs:comment "Description of the A sharp major key.";
	tonality:tonic note:As;
	tonality:degree [ a tonality:Degree;
			tonality:degree_position 1;
			tonality:degree_name "Tonic";
			tonality:note note:As;
			tonality:owned_chord co:maj7;
			tonality:interval int:unison],	
			[ a tonality:Degree;
			tonality:degree_position 2;
			tonality:degree_name "Supertonic";
			tonality:note note:C;
			tonality:owned_chord co:min7;
			tonality:interval int:second_maj],
			[ a tonality:Degree;
			tonality:degree_position 3;
			tonality:degree_name "Mediant";
			tonality:note note:D;
			tonality:owned_chord co:min7;
			tonality:interval int:third_maj],
			[ a tonality:Degree;
			tonality:degree_position 4;
			tonality:degree_name "Subdominant";
			tonality:note note:Eb;
			tonality:owned_chord co:maj7;
			tonality:interval int:fourth_per],
			[ a tonality:Degree;
			tonality:degree_position 5;
			tonality:degree_name "Dominant";
			tonality:note note:F;
			tonality:owned_chord co:seventh;
			tonality:interval int:fifth_per],
			[ a tonality:Degree;
			tonality:degree_position 6;
			tonality:degree_name "Submediant";
			tonality:note note:G;
			tonality:owned_chord co:min7;
			tonality:interval int:sixth_maj],
			[ a tonality:Degree;
			tonality:degree_position 7;
			tonality:degree_name "Subtonic or Leading Tone";
			tonality:note note:A;
			tonality:owned_chord co:hdim7;
			tonality:interval int:seventh_maj];
	.

key:Asminor
	a tonality:Key;
	rdfs:label "A sharp minor key";
	vs:term_status "testing";
	rdfs:comment "Description of the A sharp minor key.";
	tonality:tonic note:As;
	tonality:degree [ a tonality:Degree;
			tonality:degree_position 1;
			tonality:degree_name "Tonic";
			tonality:note note:As;
			tonality:owned_chord co:min7;
			tonality:interval int:unison],	
			[ a tonality:Degree;
			tonality:degree_position 2;
			tonality:degree_name "Supertonic";
			tonality:note note:Bs;
			tonality:owned_chord co:hdim7;
			tonality:interval int:second_maj],
			[ a tonality:Degree;
			tonality:degree_position 3;
			tonality:degree_name "Mediant";
			tonality:note note:Cs;
			tonality:owned_chord co:maj7;
			tonality:interval int:third_min],
			[ a tonality:Degree;
			tonality:degree_position 4;
			tonality:degree_name "Subdominant";
			rdfs:comment "This degree may appear altered borrowing the chord from the melodic minor scale.";
			tonality:note note:Ds;
			tonality:owned_chord co:min7;
			tonality:borrowed_chord co:seventh;
			tonality:interval int:fourth_per],
			[ a tonality:Degree;
			tonality:degree_position 5;
			tonality:degree_name "Dominant";
			rdfs:comment "This degree may appear altered borrowing the chord from the harmonic minor scale.";
			tonality:note note:Es;
			tonality:owned_chord co:min7;
			tonality:borrowed_chord co:seventh;
			tonality:interval int:fifth_per],
			[ a tonality:Degree;
			tonality:degree_position 6;
			tonality:degree_name "Submediant";
			tonality:note note:Fs;
			tonality:owned_chord co:maj7;
			tonality:interval int:sixth_min],
			[ a tonality:Degree;
			tonality:degree_position 7;
			tonality:degree_name "Subtonic or Leading Tone";
			tonality:note note:Gs;
			tonality:owned_chord co:seventh;
			tonality:borrowed_chord co:dim7;
			tonality:interval int:seventh_min];
	.

#B flat

key:Bbmajor
	a tonality:Key;
	rdfs:label "B flat major key";
	vs:term_status "testing";
	rdfs:comment "Description of the B flat major key.";
	tonality:tonic note:Bb;
	owl:sameAs key:Asmajor;
	.

key:Bbminor
	a tonality:Key;
	rdfs:label "B flat minor key";
	vs:term_status "testing";
	rdfs:comment "Description of the B flat minor key.";
	tonality:tonic note:Bb;
	owl:sameAs key:Asminor;
	.
#B

key:Bmajor
	a tonality:Key;
	rdfs:label "B major key";
	vs:term_status "testing";
	rdfs:comment "Description of the B major key.";
	tonality:tonic note:B;
	tonality:degree [ a tonality:Degree;
			tonality:degree_position 1;
			tonality:degree_name "Tonic";
			tonality:note note:B;
			tonality:owned_chord co:maj7;
			tonality:interval int:unison],	
			[ a tonality:Degree;
			tonality:degree_position 2;
			tonality:degree_name "Supertonic";
			tonality:note note:Cs;
			tonality:owned_chord co:min7;
			tonality:interval int:second_maj],
			[ a tonality:Degree;
			tonality:degree_position 3;
			tonality:degree_name "Mediant";
			tonality:note note:Ds;
			tonality:owned_chord co:min7;
			tonality:interval int:third_maj],
			[ a tonality:Degree;
			tonality:degree_position 4;
			tonality:degree_name "Subdominant";
			tonality:note note:E;
			tonality:owned_chord co:maj7;
			tonality:interval int:fourth_per],
			[ a tonality:Degree;
			tonality:degree_position 5;
			tonality:degree_name "Dominant";
			tonality:note note:Fs;
			tonality:owned_chord co:seventh;
			tonality:interval int:fifth_per],
			[ a tonality:Degree;
			tonality:degree_position 6;
			tonality:degree_name "Submediant";
			tonality:note note:Gs;
			tonality:owned_chord co:min7;
			tonality:interval int:sixth_maj],
			[ a tonality:Degree;
			tonality:degree_position 7;
			tonality:degree_name "Subtonic or Leading Tone";
			tonality:note note:As;
			tonality:owned_chord co:hdim7;
			tonality:interval int:seventh_maj];
	.

key:Bminor
	a tonality:Key;
	rdfs:label "B minor key";
	vs:term_status "testing";
	rdfs:comment "Description of the B minor key.";
	tonality:tonic note:B;
	tonality:degree [ a tonality:Degree;
			tonality:degree_position 1;
			tonality:degree_name "Tonic";
			tonality:note note:B;
			tonality:owned_chord co:min7;
			tonality:interval int:unison],	
			[ a tonality:Degree;
			tonality:degree_position 2;
			tonality:degree_name "Supertonic";
			tonality:note note:Cs;
			tonality:owned_chord co:hdim7;
			tonality:interval int:second_maj],
			[ a tonality:Degree;
			tonality:degree_position 3;
			tonality:degree_name "Mediant";
			tonality:note note:D;
			tonality:owned_chord co:maj7;
			tonality:interval int:third_min],
			[ a tonality:Degree;
			tonality:degree_position 4;
			tonality:degree_name "Subdominant";
			rdfs:comment "This degree may appear altered borrowing the chord from the melodic minor scale.";
			tonality:note note:E;
			tonality:owned_chord co:min7;
			tonality:borrowed_chord co:seventh;
			tonality:interval int:fourth_per],
			[ a tonality:Degree;
			tonality:degree_position 5;
			tonality:degree_name "Dominant";
			rdfs:comment "This degree may appear altered borrowing the chord from the harmonic minor scale.";
			tonality:note note:Fs;
			tonality:owned_chord co:min7;
			tonality:borrowed_chord co:seventh;
			tonality:interval int:fifth_per],
			[ a tonality:Degree;
			tonality:degree_position 6;
			tonality:degree_name "Submediant";
			tonality:note note:G;
			tonality:owned_chord co:maj7;
			tonality:interval int:sixth_min],
			[ a tonality:Degree;
			tonality:degree_position 7;
			tonality:degree_name "Subtonic or Leading Tone";
			tonality:note note:A;
			tonality:owned_chord co:seventh;
			tonality:borrowed_chord co:dim7;
			tonality:interval int:seventh_min];
	.

#B SHARP

key:Bsmajor
	a tonality:Key;
	rdfs:label "B sharp major key";
	vs:term_status "testing";
	rdfs:comment "Description of the B sharp major key.";
	tonality:tonic note:Bs;
	owl:sameAs key:Cmajor;
	.

key:Bsminor
	a tonality:Key;
	rdfs:label "B sharp minor key";
	vs:term_status "testing";
	rdfs:comment "Description of the B sharp minor key.";
	tonality:tonic note:Bs;
	owl:sameAs key:Cminor;
	.

#Tonality ontology#
