@prefix owl: <http://www.w3.org/2002/07/owl#>.
@prefix rdf: <http://www.w3.org/1999/02/22-rdf-syntax-ns#>.
@prefix rdfs: <http://www.w3.org/2000/01/rdf-schema#>.
@prefix xsd: <http://www.w3.org/2001/XMLSchema#>.
@prefix foaf: <http://xmlns.com/foaf/0.1/>.
@prefix vs: <http://www.w3.org/2003/06/sw-vocab-status/ns#>.
@prefix tl: <http://purl.org/NET/c4dm/timeline.owl#>.
@prefix event: <http://purl.org/NET/c4dm/event.owl#>.
@prefix mo: <http://purl.org/ontology/mo/>.
@prefix tonality: <http://purl.org/ontology/tonality/>.
@prefix tuning: <http://purl.org/ontology/tuning/>.
@prefix dc: <http://purl.org/dc/elements/1.1/>.
@prefix note: <http://purl.org/ontology/chord/note/>.

<> 
	a owl:Ontology;
	dc:title "The Tuning ontology";
	rdfs:label "The Tuning ontology";
	dc:description """
		Ontology describing musical instruments tuning, band tunings and musical tuning systems
	""";
	dc:creator "David Pastor Escuredo";
        foaf:maker "David Pastor Escuredo";
        dc:date "$Date: 2008/03/21 13:05:11 $";
	.

# People
#"David Pastor Escuredo" a foaf:Person.

# Status of terms
vs:term_status a owl:AnnotationProperty.

#TUNING ONTOLOGY CLASSES

tuning:TuningSystem
	a owl:Class;
	rdfs:label "Tuning System";
	rdfs:comment """
		Class representing the tuning of the octave
	""";
	vs:term_status "unstable";
	.

tuning:EqualTemperament
	a owl:Class;
	rdfs:subClassOf tuning:TuningSystem;
	rdfs:label "Equal Temperament";
	rdfs:comment """
		Temperament adjusts the intervals of the octave diving it in equal steps
	""";
	vs:term_status "unstable";
	.

tuning:WellTemperament
	a owl:Class;
	rdfs:subClassOf tuning:TuningSystem;
	rdfs:label "Well Temperament";
	rdfs:comment """
		Temperament adjusts the intervals of the octave so the progression of interval is circular but not through equal intervals
	""";
	vs:term_status "unstable";
	.

tuning:JustIntonation
	a owl:Class;
	rdfs:subClassOf tuning:TuningSystem;
	rdfs:label "Just Intonation";
	rdfs:comment """
		Tuning system where intervals are just related by rationale number ratios
	""";
	vs:term_status "unstable";
	.

tuning:Tuning
	a owl:Class;
	rdfs:label "Tuning";
	rdfs:comment """
		Class representing the specific tuning 
	""";
	vs:term_status "unstable";
	.

tuning:InstrumentTuning
	a owl:Class;
	rdfs:label "Instrument Tuning";
	rdfs:comment """
		Class representing the specific tuning of an instrument
	""";
	vs:term_status "unstable";
	.

#TUNING ONTOLOGY PROPERTIES

tuning:octave_divisions
	a owl:FunctionalProperty;
	rdfs:label "octave divisions";
	rdfs:comment """
		Number of divisions within the octave.
	""";
	rdfs:domain tuning:TuningSystem;
	rdfs:range xsd:integer;
	vs:term_status "unstable";
	.

tuning:frequency_A
	a owl:FunctionalProperty;
	rdfs:label "frequency for A";
	rdfs:comment """
		Tuning of an instrument given the exact frequency for A
	""";
	rdfs:domain tuning:Tuning;
	rdfs:range xsd:decimal;
	vs:term_status "unstable";
	.	

#TUNING SYSTEM INDIVIDUALS

tuning:twelve_edo
	a tuning:EqualTemperament;
	rdfs:label "12 EDO";
	rdfs:comment """
		12 equal division of the octave. Kind of TET
	""";
	vs:term_status "unstable";
	tuning:octave_divisons 12;
	.

tuning:meantone
	a tuning:JustIntonation;
	rdfs:label "Meantone Temperament";
	rdfs:comment """
		The meantone temperament (just intonation)
	""";
	vs:term_status "unstable";
	.
